Rewrite tail-recursive functions in terms of tailrec
The point is that it's easier to prove div specs about functions where
it's easy to isolate the effects of a single loop iterations. Functions
on tailrec form satisfy this.

We only care about tail-recursive functions because if your function ain't
tail-recursive, it will not actually diverge but run out of stack.

characteristic/cfDivScript.sml
@@ -23,6 +23,1120 @@ fun append_prog tm = let
   val tm = QCONV EVAL tm |> concl |> rand
   in ml_translatorLib.ml_prog_update (ml_progLib.add_prog tm I) end
 
+val tailrec_clos = cfTacticsLib.process_topdecs `
+  fun tailrec f x =
+    case f x of
+      Inl x => tailrec f x
+    | Inr y => y;
+  ` |> rator |> rand |> rand
+
+val tailrec_body = tailrec_clos |> rator |> rand |> rand |> rand |> rand
+
+val mk_inl_def = Define `mk_inl e =
+  Let (SOME "x") e (Con(SOME(Short "Inl")) [Var(Short "x")])`
+
+val mk_inr_def = Define `mk_inr e =
+  Let (SOME "x") e (Con(SOME(Short "Inr")) [Var(Short "x")])`
+
+val dest_opapp_exp_size = Q.store_thm("dest_opapp_exp_size",
+  `!tm f arg. dest_opapp tm = SOME(f,arg)
+   ==> exps_size arg < exp_size tm`,
+  ho_match_mp_tac cfNormaliseTheory.dest_opapp_ind
+  >> rw[cfNormaliseTheory.dest_opapp_def]
+  >> every_case_tac >> fs[]
+  >> rveq
+  >> fs[terminationTheory.size_abbrevs,astTheory.exp_size_def]
+  >> first_x_assum dxrule
+  >> fs[REWRITE_RULE [terminationTheory.size_abbrevs] terminationTheory.exps_size_thm,
+        SUM_APPEND]);
+
+val mk_single_app_def = tDefine "mk_single_app"
+  `(mk_single_app fname allow_fname (Raise e) =
+    do
+      e <- mk_single_app fname F e;
+      SOME(Raise e)
+    od) /\
+   (mk_single_app fname allow_fname (Handle e pes) =
+    do
+      e <- mk_single_app fname F e;
+      pes <- mk_single_appps fname allow_fname pes;
+      if allow_fname then
+        SOME(Handle (mk_inr e) pes)
+      else
+        SOME(Handle e pes)
+    od) /\
+   (mk_single_app fname allow_fname (Lit l) =
+    if allow_fname then
+      SOME(mk_inr(Lit l))
+    else
+      SOME(Lit l)) /\
+   (mk_single_app fname allow_fname (Con c es) =
+    do
+      es <- mk_single_apps fname F es;
+      if allow_fname then
+        SOME(mk_inr(Con c es))
+      else
+        SOME(Con c es)
+    od
+   ) /\
+   (mk_single_app fname allow_fname (Var(Short v)) =
+    if SOME v = fname then
+      NONE
+    else if allow_fname then
+      SOME(mk_inr(Var(Short v)))
+    else
+      SOME(Var(Short v))
+   ) /\
+   (mk_single_app fname allow_fname (Var v) =
+    if allow_fname then
+      SOME(mk_inr(Var v))
+    else
+      SOME(Var v)
+   ) /\
+   (mk_single_app fname allow_fname (Fun x e) =
+    let fname' = if SOME x = fname then
+                   NONE
+                 else
+                   fname
+    in
+    do
+      e <- mk_single_app fname' F e;
+      if allow_fname then
+        SOME(mk_inr(Fun x e))
+      else
+        SOME(Fun x e)
+    od
+   ) /\
+   (mk_single_app fname allow_fname (Log lop e1 e2) =
+    do
+      e1 <- mk_single_app fname F e1;
+      e2 <- mk_single_app fname F e2;
+      if allow_fname then
+        SOME(mk_inr(Log lop e1 e2))
+      else
+        SOME(Log lop e1 e2)
+    od
+   ) /\
+   (mk_single_app fname allow_fname (If e1 e2 e3) =
+    do
+      e1 <- mk_single_app fname F e1;
+      e2 <- mk_single_app fname allow_fname e2;
+      e3 <- mk_single_app fname allow_fname e3;
+      SOME(If e1 e2 e3)
+    od
+   ) /\
+   (mk_single_app fname allow_fname (Mat e pes) =
+    do
+      e <- mk_single_app fname F e;
+      pes <- mk_single_appps fname allow_fname pes;
+      SOME(Mat e pes)
+    od
+   ) /\
+   (mk_single_app fname allow_fname (Tannot e ty) =
+    do
+      e <- mk_single_app fname allow_fname e;
+      SOME(Tannot e ty)
+    od
+   ) /\
+   (mk_single_app fname allow_fname (Lannot e l) =
+    do
+      e <- mk_single_app fname allow_fname e;
+      SOME(Lannot e l)
+    od
+   ) /\
+   (mk_single_app fname allow_fname (Let NONE e1 e2) =
+    do
+      e1 <- mk_single_app fname F e1;
+      e2 <- mk_single_app fname allow_fname e2;
+      SOME(Let NONE e1 e2)
+    od) /\
+   (mk_single_app fname allow_fname (Let (SOME x) e1 e2) =
+    let fname' =
+        if SOME x = fname then
+          NONE
+        else fname
+    in
+    do
+      e1 <- mk_single_app fname F e1;
+      e2 <- mk_single_app fname' allow_fname e2;
+      SOME(Let (SOME x) e1 e2)
+    od) /\
+   (mk_single_app fname allow_fname (Letrec recfuns e) =
+    let fname' = if EXISTS ($= fname o SOME) (MAP FST recfuns)
+                 then NONE else fname
+    in
+    do
+      recfuns <- mk_single_appr fname' F recfuns;
+      e <- mk_single_app fname' allow_fname e;
+      SOME(Letrec recfuns e)
+    od) /\
+   (mk_single_app fname allow_fname (App op es) =
+      (case dest_opapp (App op es) of
+         SOME(Var(Short f),[arg]) =>
+           if SOME f = fname then
+             if allow_fname then
+               do
+                 arg <- mk_single_app fname F arg;
+                 SOME(mk_inl arg)
+               od
+             else NONE
+           else
+             do
+               arg <- mk_single_app fname F arg;
+               if allow_fname then
+                 SOME(mk_inr(App op [Var(Short f); arg]))
+               else
+                 SOME(App op [Var(Short f); arg])
+             od
+       | _ =>
+         do
+           es <- mk_single_apps fname F es;
+           if allow_fname then
+             SOME(mk_inr(App op es))
+           else
+             SOME(App op es)
+         od
+      )
+   ) /\
+   (mk_single_apps fname allow_fname (e::es) =
+    do
+      e <- mk_single_app fname allow_fname e;
+      es <- mk_single_apps fname allow_fname es;
+      SOME(e::es)
+    od) /\
+   (mk_single_apps fname allow_fname [] =
+    SOME []) /\
+   (mk_single_appps fname allow_fname ((p,e)::pes) =
+    let fname' = if EXISTS ($= fname o SOME) (pat_bindings p [])
+                 then NONE
+                 else fname
+    in
+    do
+      e <- mk_single_app fname' allow_fname e;
+      pes <- mk_single_appps fname allow_fname pes;
+      SOME((p,e)::pes)
+    od) /\
+   (mk_single_appps fname allow_fname [] =
+    SOME []) /\
+   (mk_single_appr fname allow_fname ((f,x,e)::recfuns) =
+    let fname' = if SOME x = fname then NONE else fname
+    in
+    do
+      e <- mk_single_app fname allow_fname e;
+      recfun <- mk_single_appr fname allow_fname recfuns;
+      SOME((f,x,e)::recfuns)
+    od) /\
+   (mk_single_appr fname allow_fname [] =
+    SOME [])`
+  (WF_REL_TAC `inv_image $< (\x. case x of INL (t,x,e) => exp_size e
+                                        | INR (INL (t,x,es)) => exps_size es
+                                        | INR (INR (INL (t,x,pes))) => pes_size pes
+                                        | INR (INR (INR (t,x,recfuns))) => funs_size recfuns)` >>
+   srw_tac [ARITH_ss] [terminationTheory.size_abbrevs, astTheory.exp_size_def] >>
+   imp_res_tac dest_opapp_exp_size >>
+   fs[terminationTheory.size_abbrevs,astTheory.exp_size_def]);
+
+val mk_single_app_ind = fetch "-" "mk_single_app_ind"
+
+val mk_tailrec_closure_def = Define
+  `(mk_tailrec_closure (Recclosure env [(fname,farg,fbody)] name2) =
+    do
+     gbody <- mk_single_app (SOME fname) T fbody;
+     SOME(Closure (env with <| v :=
+            (let benv = build_rec_env [(fname,farg,fbody)] env env.v
+             in nsBind fname (Closure (env with v := benv) farg gbody) env.v) |>) farg  
+          (App Opapp
+               [App Opapp
+                  [Letrec ^tailrec_clos (Var(Short "tailrec"));
+                   Var(Short fname)];
+                Var(Short farg)]
+          )
+         )
+    od) /\ mk_tailrec_closure _ = NONE`
+
+val dest_opapp_eq_nil_IMP = Q.store_thm("dest_opapp_eq_nil_IMP",
+  `dest_opapp(exp) = SOME(f,[])
+   ==> F`,
+  Cases_on `exp` >>
+  fs[cfNormaliseTheory.dest_opapp_def] >>
+  rename1 `App op exps` >>
+  Cases_on `op` >> Cases_on `exps` >>
+  fs[cfNormaliseTheory.dest_opapp_def] >>
+  every_case_tac >> fs[] >> strip_tac);
+
+val dest_opapp_eq_single_IMP = Q.store_thm("dest_opapp_eq_single_IMP",
+  `dest_opapp(App op exps) = SOME(f,[arg])
+   ==> op = Opapp /\ exps = [f;arg]`,
+  Cases_on `op` >> Cases_on `exps` >>
+  fs[cfNormaliseTheory.dest_opapp_def] >>
+  every_case_tac >> fs[] >> strip_tac >>
+  rveq >> rename1 `dest_opapp exp` >>
+  Cases_on `exp` >> fs[cfNormaliseTheory.dest_opapp_def] >>
+  rename1 `App op exps` >>
+  Cases_on `op` >> Cases_on `exps` >>  
+  fs[cfNormaliseTheory.dest_opapp_def] >>
+  every_case_tac >> fs[]);
+
+val mk_single_app_F_unchanged_gen = Q.prove(
+  `(!fname allow_fname e e'. mk_single_app fname allow_fname e = SOME e'
+               /\ allow_fname = F ==> e = e') /\
+   (!fname allow_fname es es'. mk_single_apps fname allow_fname es = SOME es'
+               /\ allow_fname = F ==> es = es') /\
+   (!fname allow_fname pes pes'. mk_single_appps fname allow_fname pes = SOME pes'
+                /\ allow_fname = F ==> pes = pes') /\
+   (!fname allow_fname recfuns recfuns'. mk_single_appr fname allow_fname recfuns = SOME recfuns'
+                /\ allow_fname = F ==> recfuns = recfuns')
+  `,
+  ho_match_mp_tac mk_single_app_ind >>
+  rw[mk_single_app_def] >> fs[] >>
+  every_case_tac >> fs[] >> rfs[] >>
+  first_x_assum drule >> simp[] >>
+  imp_res_tac dest_opapp_eq_single_IMP >>
+  fs[]);
+
+val mk_single_app_F_unchanged = save_thm("mk_single_app_F_unchanged",
+  SIMP_RULE std_ss [] mk_single_app_F_unchanged_gen);
+
+val mk_inr_res_def = Define `
+  (mk_inr_res(Rval vs) =
+   Rval(MAP (λv. Conv (SOME (TypeStamp "Inr" 4)) [v]) vs)
+  ) /\
+  (mk_inr_res res = res)`
+
+val mk_inl_res_def = Define `
+  (mk_inl_res(Rval vs) =
+   Rval(MAP (λv. Conv (SOME (TypeStamp "Inl" 4)) [v]) vs)
+  ) /\
+  (mk_inl_res res = res)`
+
+val dest_inr_v_def = Define `
+  (dest_inr_v (Conv (SOME (TypeStamp txt n)) [v]) =
+   if txt = "Inr" /\ n = 4 then
+     SOME v
+   else
+     NONE) /\
+  (dest_inr_v _ = NONE)`
+
+val dest_inl_v_def = Define `
+  (dest_inl_v (Conv (SOME (TypeStamp txt n)) [v]) =
+   if txt = "Inl" /\ n = 4 then
+     SOME v
+   else
+     NONE) /\
+  (dest_inl_v _ = NONE)`
+
+val dest_inr_v_IMP = Q.store_thm("dest_inr_v_IMP",
+  `!e1 v. dest_inr_v e1 = SOME v ==> e1 = Conv (SOME (TypeStamp "Inr" 4)) [v]`,
+  ho_match_mp_tac (fetch "-" "dest_inr_v_ind") >>
+  rw[dest_inr_v_def]);
+
+val dest_inl_v_IMP = Q.store_thm("dest_inl_v_IMP",
+  `!e1 v. dest_inl_v e1 = SOME v ==> e1 = Conv (SOME (TypeStamp "Inl" 4)) [v]`,
+  ho_match_mp_tac (fetch "-" "dest_inl_v_ind") >>
+  rw[dest_inl_v_def]);
+
+val evaluate_inl = Q.store_thm("evaluate_inl",
+    `do_con_check env.c (SOME (Short "Inl")) 1 = T /\
+    (!v. build_conv env.c (SOME (Short "Inl")) [v] =
+           SOME(Conv (SOME (TypeStamp "Inl" 4)) [v]))
+    ==> evaluate st env [mk_inl e] =
+        case evaluate st env [e] of
+            (st,Rval v) => (st,mk_inl_res(Rval v))
+          | (st,rerr) => (st,rerr)`,
+    rw[terminationTheory.evaluate_def,mk_inl_def,namespaceTheory.nsOptBind_def,
+       ml_progTheory.nsLookup_nsBind_compute,mk_inl_res_def] >>
+    ntac 2(PURE_TOP_CASE_TAC >> fs[] >> rveq) >>
+    imp_res_tac evaluatePropsTheory.evaluate_length >>
+    fs[quantHeuristicsTheory.LIST_LENGTH_1]);
+
+val build_conv_check_IMP_nsLookup = Q.prove(
+  `!env const v consname stamp n.
+  (∀v. build_conv env (SOME const) [v] =
+   SOME (Conv (SOME stamp) [v])) /\
+  do_con_check env (SOME const) n
+  ==> nsLookup env const = SOME(n,stamp)
+  `,
+  rw[semanticPrimitivesTheory.build_conv_def,semanticPrimitivesTheory.do_con_check_def,
+     namespaceTheory.nsLookup_def] >>
+  every_case_tac >> fs[]);
+
+val evaluate_IMP_inl = Q.store_thm("evaluate_IMP_inl",
+    `do_con_check env.c (SOME (Short "Inl")) 1 = T /\
+    (!v. build_conv env.c (SOME (Short "Inl")) [v] =
+           SOME(Conv (SOME (TypeStamp "Inl" 4)) [v])) /\
+    evaluate st env [e] = (st',res)
+    ==> evaluate st env [mk_inl e] = (st',mk_inl_res res)`,
+    rw[terminationTheory.evaluate_def,mk_inl_def,namespaceTheory.nsOptBind_def,
+       ml_progTheory.nsLookup_nsBind_compute] >>
+    PURE_TOP_CASE_TAC >> fs[mk_inl_res_def] >>
+    imp_res_tac evaluatePropsTheory.evaluate_length >>
+    fs[quantHeuristicsTheory.LIST_LENGTH_1]);
+
+val evaluate_inr = Q.store_thm("evaluate_inr",
+    `do_con_check env.c (SOME (Short "Inr")) 1 = T /\
+    (!v. build_conv env.c (SOME (Short "Inr")) [v] =
+           SOME(Conv (SOME (TypeStamp "Inr" 4)) [v]))
+    ==> evaluate st env [mk_inr e] =
+        case evaluate st env [e] of
+            (st,Rval v) => (st,mk_inr_res(Rval v))
+          | (st,rerr) => (st,rerr)`,
+    rw[terminationTheory.evaluate_def,mk_inr_def,namespaceTheory.nsOptBind_def,
+       ml_progTheory.nsLookup_nsBind_compute,mk_inr_res_def] >>
+    ntac 2(PURE_TOP_CASE_TAC >> fs[] >> rveq) >>
+    imp_res_tac evaluatePropsTheory.evaluate_length >>
+    fs[quantHeuristicsTheory.LIST_LENGTH_1]);
+
+val st = ``st:'ffi semanticPrimitives$state``
+
+val evaluate_IMP_inr = Q.store_thm("evaluate_IMP_inr",
+    `do_con_check env.c (SOME (Short "Inr")) 1 = T /\
+    (!v. build_conv env.c (SOME (Short "Inr")) [v] =
+           SOME(Conv (SOME (TypeStamp "Inr" 4)) [v])) /\
+    evaluate ^st env [e] = (st',res)
+    ==> evaluate st env [mk_inr e] = (st',mk_inr_res res)`,
+    rw[terminationTheory.evaluate_def,mk_inr_def,namespaceTheory.nsOptBind_def,
+       ml_progTheory.nsLookup_nsBind_compute] >>
+    PURE_TOP_CASE_TAC >> fs[mk_inr_res_def] >>
+    imp_res_tac evaluatePropsTheory.evaluate_length >>
+    fs[quantHeuristicsTheory.LIST_LENGTH_1]);
+
+val mk_single_app_NONE_evaluate = Q.prove(
+  `(!^st env es es'. mk_single_apps NONE T es = SOME es'
+    /\ do_con_check env.c (SOME (Short "Inr")) 1 = T
+    /\ (!v. build_conv env.c (SOME (Short "Inr")) [v] =
+           SOME(Conv (SOME (TypeStamp "Inr" 4)) [v]))
+    ==> evaluate st env es'
+        = case evaluate st env es of
+           (st',res) => (st', mk_inr_res res)
+   ) /\
+   (!^st env v pes err_v pes'. mk_single_appps NONE T pes = SOME pes'
+    /\ do_con_check env.c (SOME (Short "Inr")) 1 = T
+    /\ (!v. build_conv env.c (SOME (Short "Inr")) [v] =
+           SOME(Conv (SOME (TypeStamp "Inr" 4)) [v]))
+    ==> evaluate_match st env v pes' err_v
+        = case evaluate_match st env v pes err_v of
+           (st',res) => (st', mk_inr_res res)
+   )
+   `,
+  ho_match_mp_tac terminationTheory.evaluate_ind >> rpt strip_tac >> PURE_TOP_CASE_TAC
+  (* Nil *)
+  >- (fs[mk_single_app_def] >> rveq >> fs[terminationTheory.evaluate_def,mk_inr_res_def])
+  (* Sequence *)
+  >- (fs[Once terminationTheory.evaluate_def,mk_single_app_def] >>
+      rveq >> every_case_tac >>
+      fs[] >> rveq >> fs[PULL_EXISTS] >>
+      rpt(first_x_assum drule) >> rpt(disch_then drule) >> rpt strip_tac >>
+      simp[Once terminationTheory.evaluate_def] >>
+      fs[mk_inr_res_def] >>
+      imp_res_tac evaluatePropsTheory.evaluate_length >>
+      fs[quantHeuristicsTheory.LIST_LENGTH_1])
+  (* Lit *)
+  >- (fs[mk_single_app_def] >> rveq >> fs[evaluate_IMP_inr])
+  (* Raise *)
+  >- (fs[mk_single_app_def] >> rveq >> fs[evaluate_IMP_inr] >> fs[terminationTheory.evaluate_def] >>
+      imp_res_tac mk_single_app_F_unchanged >> rveq >>
+      every_case_tac >> fs[] >> rveq >> fs[mk_inr_res_def])
+  (* Handle *)
+  >- (fs[mk_single_app_def] >> rveq >> fs[Once terminationTheory.evaluate_def] >>
+      imp_res_tac mk_single_app_F_unchanged >> rveq >>            
+      every_case_tac >> fs[] >> rveq >>
+      rfs[evaluate_inr] >> fs[mk_inr_res_def] >>
+      rveq >> fs[])
+  (* Con *)
+  >- (fs[mk_single_app_def] >> rveq >>
+      imp_res_tac mk_single_app_F_unchanged >> rveq >>
+      fs[evaluate_IMP_inr])
+  (* Var*)
+  >- (rename1 `Var n` >> Cases_on `n` >>
+      fs[mk_single_app_def] >> rveq >>
+      fs[evaluate_IMP_inr])
+  (* Fun *)
+  >- (fs[mk_single_app_def] >> rveq >>
+      imp_res_tac mk_single_app_F_unchanged >> rveq >>
+      fs[evaluate_IMP_inr])
+  (* App *)
+  >- (fs[mk_single_app_def] >>
+      reverse(Cases_on `op = Opapp`)
+      >- (Cases_on `op` >>
+          rveq >> fs[cfNormaliseTheory.dest_opapp_def] >>
+          rveq >> simp[evaluate_IMP_inr] >>
+          imp_res_tac mk_single_app_F_unchanged >> rveq >>
+          simp[] >> every_case_tac >> fs[mk_inr_res_def] >>
+          rfs[] >>  imp_res_tac evaluatePropsTheory.evaluate_length >>
+          fs[quantHeuristicsTheory.LIST_LENGTH_1] >> rveq >>
+          rfs[] >> fs[evaluate_IMP_inr]
+         ) >>
+      rveq >>
+      Cases_on `es`
+      >- (fs[cfNormaliseTheory.dest_opapp_def] >>
+          rveq >> simp[evaluate_IMP_inr] >>
+          imp_res_tac mk_single_app_F_unchanged >> rveq >>
+          simp[] >> every_case_tac >> fs[mk_inr_res_def] >>
+          rfs[] >>  imp_res_tac evaluatePropsTheory.evaluate_length >>
+          fs[quantHeuristicsTheory.LIST_LENGTH_1] >> rveq >>
+          rfs[] >> fs[evaluate_IMP_inr]) >>
+      rename1 `dest_opapp (App Opapp (exp::exps))` >>
+      reverse(Cases_on `exps`)
+      >- (fs[cfNormaliseTheory.dest_opapp_def] >>
+          simp[] >> rpt(PURE_FULL_CASE_TAC >> fs[] >> rveq) >>
+          fs[mk_single_app_def] >> rveq >>
+          imp_res_tac mk_single_app_F_unchanged >> rveq >>
+          fs[evaluate_IMP_inr] >>
+          fs[mk_inr_def] >>
+          simp[] >> simp[terminationTheory.evaluate_def] >>
+          PURE_TOP_CASE_TAC >> fs[mk_inr_res_def] >>
+          rfs[] >>  imp_res_tac evaluatePropsTheory.evaluate_length >>
+          fs[quantHeuristicsTheory.LIST_LENGTH_1] >> rveq >>
+          rfs[] >>
+          imp_res_tac dest_opapp_eq_nil_IMP) >>
+      fs[cfNormaliseTheory.dest_opapp_def] >>
+      rveq >>
+      imp_res_tac mk_single_app_F_unchanged >> rveq >>
+      simp[evaluate_IMP_inr])
+  (* Log *)
+  >- (fs[mk_single_app_def] >> rveq >>
+      imp_res_tac mk_single_app_F_unchanged >> rveq >>
+      simp[evaluate_IMP_inr])
+  (* If *)
+  >- (fs[mk_single_app_def] >> rveq >>
+      imp_res_tac mk_single_app_F_unchanged >> rveq >>
+      fs[Once terminationTheory.evaluate_def] >>
+      TOP_CASE_TAC >> reverse TOP_CASE_TAC >-
+        (fs[] >> rveq >> fs[mk_inr_res_def]) >>
+      fs[semanticPrimitivesTheory.do_if_def] >>
+      rw[] >> fs[] >>
+      rveq >> fs[mk_inr_res_def])
+  (* Mat *)
+  >- (fs[mk_single_app_def] >> rveq >>
+      imp_res_tac mk_single_app_F_unchanged >> rveq >>
+      fs[Once terminationTheory.evaluate_def] >>
+      TOP_CASE_TAC >> reverse TOP_CASE_TAC >-
+        (fs[] >> rveq >> fs[mk_inr_res_def]) >>
+      fs[])
+  (* Let *)
+  >- (rename1 `Let xo` >> Cases_on `xo` >>
+      fs[mk_single_app_def] >> rveq >>
+      imp_res_tac mk_single_app_F_unchanged >> rveq >>
+      fs[Once terminationTheory.evaluate_def] >>
+      TOP_CASE_TAC >> reverse TOP_CASE_TAC >-
+        (fs[] >> rveq >> fs[mk_inr_res_def]) >>
+      fs[] >> rveq >> fs[mk_inr_res_def])
+  (* Letrec *)
+  >- (fs[mk_single_app_def] >> rveq >>
+      imp_res_tac mk_single_app_F_unchanged >> rveq >>
+      fs[Once terminationTheory.evaluate_def] >>
+      rw[] >> fs[] >> rveq >> fs[mk_inr_res_def])
+  (* Tannot *)
+  >- (fs[mk_single_app_def] >> rveq >>
+      fs[Once terminationTheory.evaluate_def])
+  (* Lannot *)
+  >- (fs[mk_single_app_def] >> rveq >>
+      fs[Once terminationTheory.evaluate_def])
+  (* Pmatch empty row *)
+  >- (fs[mk_single_app_def] >> rveq >>
+      fs[terminationTheory.evaluate_def] >> rveq >>
+      fs[mk_inr_res_def])
+  (* Pmatch cons *)
+  >- (fs[mk_single_app_def] >> rveq >>
+      fs[Once terminationTheory.evaluate_def] >> rveq >>
+      reverse IF_CASES_TAC >-
+        (fs[] >> rveq >> fs[mk_inr_res_def]) >>
+      fs[] >> TOP_CASE_TAC >>
+      fs[] >> rveq >> fs[mk_inr_res_def])
+  );
+
+val mk_single_app_NONE_evaluate_single = Q.prove(
+  `(!^st env e e'. mk_single_app NONE T e = SOME e'
+    /\ do_con_check env.c (SOME (Short "Inr")) 1
+    /\ (!v. build_conv env.c (SOME (Short "Inr")) [v] =
+           SOME(Conv (SOME (TypeStamp "Inr" 4)) [v]))
+    ==> evaluate st env [e']
+        = case evaluate st env [e] of
+           (st',res) => (st', mk_inr_res res)
+   )`,
+  rpt strip_tac >>
+  match_mp_tac(CONJUNCT1 mk_single_app_NONE_evaluate) >>
+  simp[mk_single_app_def]);
+
+val nsLookup_build_rec_env_fresh = Q.prove(
+ `!funs env env' fname.
+  EVERY (λx. fname ≠ x) (MAP FST funs)
+  ==>
+  nsLookup(build_rec_env funs env' env.v) (Short fname) =
+  nsLookup env.v (Short fname)`,
+  `∀(funs:(string # string # exp) list) funs' env env' fname.
+   EVERY (λx. fname ≠ x) (MAP FST funs) ⇒
+   nsLookup
+   (FOLDR (λ(f,x,e) env''. nsBind f (Recclosure env' (funs':(string # string # exp) list) f) env'')
+          env.v funs) (Short fname) = nsLookup env.v (Short fname)`
+    suffices_by rw[semanticPrimitivesTheory.build_rec_env_def] >>
+  Induct >> rw[semanticPrimitivesTheory.build_rec_env_def] >>
+  fs[ELIM_UNCURRY]);
+
+val nsLookup_alist_to_ns_fresh = Q.prove(
+ `!l fname.
+  EVERY (λx. fname ≠ x) (MAP FST l)
+  ==>
+  nsLookup(alist_to_ns l) (Short fname) = NONE`,
+  fs[namespaceTheory.alist_to_ns_def,namespaceTheory.nsLookup_def,ALOOKUP_NONE,EVERY_MEM]);
+
+val partially_evaluates_to_def = Define `
+partially_evaluates_to fv env st [] = T /\
+partially_evaluates_to fv env st ((e1,e2)::r) =
+  case evaluate st env [e1] of
+    (st',Rval v1) =>
+      (?v. dest_inr_v(HD v1) = SOME v /\ evaluate st env [e2] = (st',Rval [v]) /\
+           partially_evaluates_to fv env st' r)
+      \/
+      (?v st'' res. dest_inl_v(HD v1) = SOME v /\ evaluate st env [e2] = (st'',res) /\
+          case do_opapp [fv;v] of
+            SOME(env',e3) =>
+               if st'.clock = 0 then st'' = st' /\ res = Rerr(Rabort(Rtimeout_error))
+               else
+                 evaluate (dec_clock st') env' [e3] = (st'',res) /\
+                 (case res of Rval _ =>
+                    partially_evaluates_to fv env st'' r
+                  | _ => T)
+          | NONE => res = Rerr (Rabort Rtype_error))
+   | (st',rerr) => evaluate st env [e2] = (st',rerr)
+`
+
+val partially_evaluates_to_match_def = Define `
+partially_evaluates_to_match fv mv err_v env st (pr1,pr2) =
+  case evaluate_match st env mv pr1 err_v of
+    (st',Rval v1) =>
+      (?v. dest_inr_v(HD v1) = SOME v /\ evaluate_match st env mv pr2 err_v = (st',Rval [v]))
+      \/
+      (?v st'' res. dest_inl_v(HD v1) = SOME v /\ evaluate_match st env mv pr2 err_v = (st'',res) /\
+          case do_opapp [fv;v] of
+              SOME(env',e3) =>
+                if st'.clock = 0 then (st'' = st' /\ res = Rerr(Rabort(Rtimeout_error)))
+                else              
+                   evaluate (dec_clock st') env' [e3] = (st'',res)
+            | NONE => res = Rerr (Rabort Rtype_error))
+   | (st',rerr) => evaluate_match st env mv pr2 err_v = (st',rerr)
+`
+
+val mk_single_app_evaluate = Q.prove(
+  `(!^st env es es' fname fv. mk_single_apps (SOME fname) T es = SOME es'
+    /\ do_con_check env.c (SOME (Short "Inr")) 1 = T
+    /\ (!v. build_conv env.c (SOME (Short "Inr")) [v] =
+           SOME(Conv (SOME (TypeStamp "Inr" 4)) [v]))
+    /\ do_con_check env.c (SOME (Short "Inl")) 1 = T
+    /\ (!v. build_conv env.c (SOME (Short "Inl")) [v] =
+           SOME(Conv (SOME (TypeStamp "Inl" 4)) [v]))
+    /\ nsLookup env.v (Short fname) = SOME fv
+    ==> partially_evaluates_to fv env st (ZIP(es',es))
+   ) /\
+   (!^st env v pes err_v pes' fname fv. mk_single_appps (SOME fname) T pes = SOME pes'
+    /\ do_con_check env.c (SOME (Short "Inr")) 1 = T
+    /\ (!v. build_conv env.c (SOME (Short "Inr")) [v] =
+           SOME(Conv (SOME (TypeStamp "Inr" 4)) [v]))
+    /\ do_con_check env.c (SOME (Short "Inl")) 1 = T
+    /\ (!v. build_conv env.c (SOME (Short "Inl")) [v] =
+           SOME(Conv (SOME (TypeStamp "Inl" 4)) [v]))
+    /\ nsLookup env.v (Short fname) = SOME fv
+    ==> partially_evaluates_to_match fv v err_v env st (pes',pes)
+   )
+   `,
+  ho_match_mp_tac terminationTheory.evaluate_ind >> rpt strip_tac
+  (* Nil *)
+  >- (fs[mk_single_app_def] >> rveq >> fs[partially_evaluates_to_def])
+  (* Sequence *)
+  >- (fs[mk_single_app_def] >>
+      rveq >> fs[partially_evaluates_to_def,ZIP] >>
+      TOP_CASE_TAC >> TOP_CASE_TAC >>
+      fs[PULL_EXISTS] >>
+      rpt(first_x_assum drule >> rpt(disch_then drule) >> rpt strip_tac) >>
+      rfs[partially_evaluates_to_def]
+      >- (first_x_assum drule >> rpt(disch_then drule) >> fs[]) >>
+      disj2_tac >>
+      ntac 4 (TOP_CASE_TAC >> fs[]) >> metis_tac[])
+  (* Lit *)
+  >- (fs[mk_single_app_def] >> rveq >>
+      fs[partially_evaluates_to_def,evaluate_inr] >>
+      fs[terminationTheory.evaluate_def,mk_inr_res_def,dest_inr_v_def])
+  (* Raise *)
+  >- (fs[mk_single_app_def] >> rveq >>
+      fs[partially_evaluates_to_def,terminationTheory.evaluate_def] >>
+      imp_res_tac mk_single_app_F_unchanged >> rveq >>
+      every_case_tac >> fs[])
+  (* Handle *)
+  >- (fs[mk_single_app_def] >> rveq >>
+      fs[partially_evaluates_to_def] >>
+      imp_res_tac mk_single_app_F_unchanged >> rveq >>
+      fs[Once terminationTheory.evaluate_def] >>
+      fs[evaluate_inr] >>
+      every_case_tac >> fs[PULL_EXISTS] >> rveq >>
+      fs[mk_inr_res_def] >> rveq >> 
+      imp_res_tac evaluatePropsTheory.evaluate_length >>
+      fs[quantHeuristicsTheory.LIST_LENGTH_1] >>
+      fs[dest_inr_v_def] >>
+      fs[terminationTheory.evaluate_def] >>
+      rpt(first_x_assum drule >> rpt(disch_then drule) >> rpt strip_tac) >>
+      rfs[partially_evaluates_to_match_def] >>
+      every_case_tac >> fs[])
+  (* Con *)
+  >- (fs[mk_single_app_def] >> rveq >>
+      imp_res_tac mk_single_app_F_unchanged >> rveq >>
+      fs[partially_evaluates_to_def] >>
+      fs[evaluate_inr] >>
+      every_case_tac >> fs[] >>
+      imp_res_tac evaluatePropsTheory.evaluate_length >>
+      fs[quantHeuristicsTheory.LIST_LENGTH_1] >>
+      fs[mk_inr_res_def] >> rveq >> fs[dest_inr_v_def])
+  (* Var*)
+  >- (rename1 `Var n` >> Cases_on `n` >>
+      fs[mk_single_app_def] >> rveq >>
+      fs[partially_evaluates_to_def] >>
+      fs[evaluate_inr] >>
+      every_case_tac >> fs[] >>
+      imp_res_tac evaluatePropsTheory.evaluate_length >>
+      fs[quantHeuristicsTheory.LIST_LENGTH_1] >>
+      fs[mk_inr_res_def] >> rveq >> fs[dest_inr_v_def])
+  (* Fun *)
+  >- (fs[mk_single_app_def] >> rveq >>
+      imp_res_tac mk_single_app_F_unchanged >> rveq >>
+      simp[partially_evaluates_to_def,evaluate_inr] >>
+      simp[terminationTheory.evaluate_def,mk_inr_res_def,dest_inr_v_def])
+  (* App *)
+  >- (fs[mk_single_app_def] >>
+      reverse(Cases_on `op = Opapp`)
+      >- (Cases_on `op` >>
+          rveq >> fs[cfNormaliseTheory.dest_opapp_def] >>
+          rveq >> simp[evaluate_inr,partially_evaluates_to_def] >>
+          imp_res_tac mk_single_app_F_unchanged >> rveq >>
+          simp[] >> every_case_tac >> fs[mk_inr_res_def] >>
+          rfs[] >>  imp_res_tac evaluatePropsTheory.evaluate_length >>
+          fs[quantHeuristicsTheory.LIST_LENGTH_1] >> rveq >>
+          rfs[] >> fs[dest_inr_v_def]) >>
+      rveq >>
+      Cases_on `es`
+      >- (fs[cfNormaliseTheory.dest_opapp_def] >>
+          rveq >> simp[partially_evaluates_to_def,evaluate_inr] >>
+          imp_res_tac mk_single_app_F_unchanged >> rveq >>
+          simp[] >> every_case_tac >> fs[mk_inr_res_def] >>
+          rfs[] >>  imp_res_tac evaluatePropsTheory.evaluate_length >>
+          fs[quantHeuristicsTheory.LIST_LENGTH_1] >> rveq >>
+          rfs[] >> fs[dest_inr_v_def]) >>
+      rename1 `dest_opapp (App Opapp (exp::exps))` >>
+      reverse(Cases_on `exps`)
+      >- (fs[cfNormaliseTheory.dest_opapp_def] >>
+          simp[] >> rpt(PURE_FULL_CASE_TAC >> fs[] >> rveq) >>
+          fs[mk_single_app_def] >> rveq >>
+          imp_res_tac mk_single_app_F_unchanged >> rveq >>
+          TRY(qmatch_goalsub_abbrev_tac `Letrec l e` >>
+              Cases_on `EXISTS ($= (SOME fname) ∘ SOME) (MAP FST l)` >>
+              FULL_SIMP_TAC std_ss [] >>
+              imp_res_tac mk_single_app_F_unchanged >> rveq >>
+              fs[partially_evaluates_to_def,evaluate_inr,evaluate_inl] >>
+              rpt(PURE_FULL_CASE_TAC >> rveq >> fs[]) >>
+              imp_res_tac evaluatePropsTheory.evaluate_length >>          
+              fs[quantHeuristicsTheory.LIST_LENGTH_1] >> rveq >>
+              fs[mk_inr_res_def] >> rveq >> fs[dest_inr_v_def]) >>
+          TRY(qmatch_goalsub_abbrev_tac `mk_inr` >>
+              fs[partially_evaluates_to_def,evaluate_inr,evaluate_inl] >>
+              rpt(PURE_FULL_CASE_TAC >> rveq >> fs[]) >>
+              imp_res_tac evaluatePropsTheory.evaluate_length >>          
+              fs[quantHeuristicsTheory.LIST_LENGTH_1] >> rveq >>
+              fs[mk_inr_res_def] >> rveq >> fs[dest_inr_v_def] >>
+              imp_res_tac dest_opapp_eq_nil_IMP) >>
+          imp_res_tac dest_opapp_eq_nil_IMP  >>
+          fs[partially_evaluates_to_def,evaluate_inl] >>
+          fs[terminationTheory.evaluate_def] >>
+          rpt(PURE_FULL_CASE_TAC >> rveq >> fs[]) >>
+          imp_res_tac evaluatePropsTheory.evaluate_length >>          
+          fs[quantHeuristicsTheory.LIST_LENGTH_1] >> rveq >>
+          fs[mk_inl_res_def] >> rveq >>
+          fs[dest_inl_v_def,dest_inr_v_def] >>
+          qmatch_goalsub_abbrev_tac `a1 = _` >>
+          MAP_EVERY qexists_tac [`FST a1`,`SND a1`] >>
+          simp[] >> PURE_TOP_CASE_TAC >> simp[]) >>      
+      fs[cfNormaliseTheory.dest_opapp_def] >>
+      rveq >>
+      imp_res_tac mk_single_app_F_unchanged >> rveq >>
+      simp[partially_evaluates_to_def,evaluate_inr] >>
+      simp[terminationTheory.evaluate_def] >>
+      every_case_tac >> fs[mk_inr_res_def] >>
+      rveq >>
+      imp_res_tac evaluatePropsTheory.evaluate_length >>
+      fs[quantHeuristicsTheory.LIST_LENGTH_1] >> rveq >>
+      fs[dest_inr_v_def])
+  (* Log *)
+  >- (fs[mk_single_app_def] >> rveq >>
+      imp_res_tac mk_single_app_F_unchanged >> rveq >>
+      simp[partially_evaluates_to_def,evaluate_inr] >>
+      every_case_tac >> fs[mk_inr_res_def] >> rfs[] >>
+      imp_res_tac evaluatePropsTheory.evaluate_length >>
+      fs[quantHeuristicsTheory.LIST_LENGTH_1] >> rveq >>
+      rfs[dest_inr_v_def])
+  (* If *)
+  >- (fs[mk_single_app_def] >> rveq >>
+      imp_res_tac mk_single_app_F_unchanged >> rveq >>
+      simp[partially_evaluates_to_def] >>
+      fs[terminationTheory.evaluate_def,semanticPrimitivesTheory.do_if_def] >>
+      Cases_on `evaluate st env [e1]` >> rename1 `(_,result)` >>
+      reverse(Cases_on `result`) >- fs[] >>
+      rw[] >> fs[] >> rfs[] >>
+      rfs[partially_evaluates_to_def,PULL_EXISTS] >>
+      rpt(first_x_assum drule >> rpt(disch_then drule) >> rpt strip_tac))
+  (* Mat *)
+  >- (fs[mk_single_app_def] >> rveq >>
+      imp_res_tac mk_single_app_F_unchanged >> rveq >>
+      simp[partially_evaluates_to_def] >>
+      Cases_on `evaluate st env [e]` >> rename1 `(_,result)` >>
+      reverse(Cases_on `result`) >- fs[terminationTheory.evaluate_def] >>            
+      fs[terminationTheory.evaluate_def,partially_evaluates_to_match_def,PULL_EXISTS] >>
+      rpt(first_x_assum drule >> rpt(disch_then drule) >> rpt strip_tac) >>
+      rpt(TOP_CASE_TAC >> fs[] >> rveq))
+  (* Let *)
+  >- (rename1 `Let xo` >> Cases_on `xo` >>
+      fs[mk_single_app_def] >> rveq >>
+      imp_res_tac mk_single_app_F_unchanged >> rveq >>
+      fs[partially_evaluates_to_def,PULL_EXISTS] >>
+      fs[terminationTheory.evaluate_def,namespaceTheory.nsOptBind_def] >>
+      Cases_on `evaluate st env [e1]` >> rename1 `(_,result)` >>
+      reverse(Cases_on `result`) >- fs[terminationTheory.evaluate_def] >>
+      rpt(first_x_assum drule >> rpt(disch_then drule) >> rpt strip_tac) >>
+      fs[] >>
+      rpt(first_x_assum drule >> rpt(disch_then drule) >> rpt strip_tac) >>
+      Cases_on `x = fname` >> fs[] >> rveq >> fs[ml_progTheory.nsLookup_nsBind_compute] >>
+      rpt(first_x_assum drule >> rpt(disch_then drule) >> rpt strip_tac) >>
+      fs[] >>      
+      drule mk_single_app_NONE_evaluate_single >>
+      qmatch_goalsub_abbrev_tac `evaluate a1 a2` >>
+      disch_then(qspecl_then [`a1`,`a2`] mp_tac) >>
+      unabbrev_all_tac >>
+      simp[] >> disch_then kall_tac >>
+      every_case_tac >> fs[mk_inr_res_def] >>
+      rveq >>
+      imp_res_tac evaluatePropsTheory.evaluate_length >>
+      fs[quantHeuristicsTheory.LIST_LENGTH_1] >>
+      rveq >> fs[dest_inr_v_def])
+  (* Letrec *)
+  >- (fs[mk_single_app_def] >> rveq >>
+      imp_res_tac mk_single_app_F_unchanged >> rveq >>
+      PURE_FULL_CASE_TAC >> FULL_SIMP_TAC std_ss [] >>
+      fs[partially_evaluates_to_def,terminationTheory.evaluate_def] >>
+      rw[] >> fs[PULL_EXISTS] >>
+      rpt(first_x_assum drule >> rpt(disch_then drule) >> rpt strip_tac) >>
+      rfs[o_DEF,nsLookup_build_rec_env_fresh,partially_evaluates_to_def] >>
+      drule mk_single_app_NONE_evaluate_single >>
+      qmatch_goalsub_abbrev_tac `evaluate a1 a2` >>
+      disch_then(qspecl_then [`a1`,`a2`] mp_tac) >>
+      unabbrev_all_tac >>
+      simp[] >> disch_then kall_tac >>
+      every_case_tac >> fs[mk_inr_res_def] >>
+      rveq >>
+      imp_res_tac evaluatePropsTheory.evaluate_length >>
+      fs[quantHeuristicsTheory.LIST_LENGTH_1] >>
+      rveq >> fs[dest_inr_v_def])
+  (* Tannot *)
+  >- (fs[mk_single_app_def] >> rveq >>
+      fs[PULL_EXISTS] >> first_x_assum drule >>
+      rpt(disch_then drule) >>
+      simp[partially_evaluates_to_def,terminationTheory.evaluate_def])
+  (* Lannot *)
+  >- (fs[mk_single_app_def] >> rveq >>
+      fs[PULL_EXISTS] >> first_x_assum drule >>
+      rpt(disch_then drule) >>
+      simp[partially_evaluates_to_def,terminationTheory.evaluate_def])
+  (* Pmatch empty row *)
+  >- (fs[mk_single_app_def] >> rveq >>
+      simp[partially_evaluates_to_match_def,terminationTheory.evaluate_def])
+  (* Pmatch cons *)
+  >- (fs[mk_single_app_def] >> rveq >>
+      PURE_FULL_CASE_TAC >> FULL_SIMP_TAC std_ss [] >>        
+      fs[partially_evaluates_to_match_def,terminationTheory.evaluate_def] >>
+      rw[] >>
+      fs[PULL_EXISTS] >>
+      Cases_on `pmatch env.c st.refs p v []` >> fs[] >>
+      rpt(first_x_assum drule >> rpt(disch_then drule) >> strip_tac) >>
+      rfs[o_DEF,partially_evaluates_to_def] >>
+      fs[ml_progTheory.nsLookup_nsAppend_Short] >>
+      imp_res_tac semanticPrimitivesPropsTheory.pmatch_extend >> rveq >>
+      rfs[] >>
+      qpat_x_assum `MAP _ _ = pat_bindings _ _` (assume_tac o GSYM) >>
+      fs[] >> rfs[nsLookup_alist_to_ns_fresh] >>
+      TRY(qmatch_asmsub_abbrev_tac `mk_single_app (SOME _) T e = SOME ea`
+          >> every_case_tac >> fs[] >> every_case_tac >> fs[]) >>
+      drule mk_single_app_NONE_evaluate_single >>
+      qmatch_goalsub_abbrev_tac `evaluate a1 a2` >>
+      disch_then(qspecl_then [`a1`,`a2`] mp_tac) >>
+      unabbrev_all_tac >>
+      simp[] >> disch_then kall_tac >>      
+      every_case_tac >> fs[mk_inr_res_def] >>
+      rveq >>
+      imp_res_tac evaluatePropsTheory.evaluate_length >>
+      fs[quantHeuristicsTheory.LIST_LENGTH_1] >>
+      qmatch_asmsub_abbrev_tac `evaluate _ _ _ = (_,result)` >>
+      Cases_on `result` >> fs[mk_inr_res_def] >> rveq >> fs[dest_inr_v_def] >>
+      imp_res_tac evaluatePropsTheory.evaluate_length >>
+      fs[quantHeuristicsTheory.LIST_LENGTH_1] >> fs[dest_inr_v_def])
+    );
+
+val mk_single_app_evaluate_single = Q.store_thm("mk_single_app_evaluate_single",
+  `!^st env e e' fname fv. mk_single_app (SOME fname) T e = SOME e'
+    /\ do_con_check env.c (SOME (Short "Inr")) 1 = T
+    /\ (!v. build_conv env.c (SOME (Short "Inr")) [v] =
+           SOME(Conv (SOME (TypeStamp "Inr" 4)) [v]))
+    /\ do_con_check env.c (SOME (Short "Inl")) 1 = T
+    /\ (!v. build_conv env.c (SOME (Short "Inl")) [v] =
+           SOME(Conv (SOME (TypeStamp "Inl" 4)) [v]))
+    /\ nsLookup env.v (Short fname) = SOME fv
+    ==> partially_evaluates_to fv env st [(e',e)]`,
+  rpt strip_tac >>
+  `mk_single_apps (SOME fname) T [e] = SOME [e']` by simp[mk_single_app_def] >>
+  drule(CONJUNCT1 mk_single_app_evaluate) >>
+  rpt(disch_then drule) >> simp[]);
+
+val evaluate_tailrec_ind_lemma = Q.prove(
+  `!ck fbody gbody env env' ^st farg x v fname st' res.
+   mk_single_app (SOME fname) T fbody = SOME gbody /\
+   do_con_check env.c (SOME (Short "Inr")) 1 /\
+   (∀v.
+        build_conv env.c (SOME (Short "Inr")) [v] =
+        SOME (Conv (SOME (TypeStamp "Inr" 4)) [v])) /\
+   do_con_check env.c (SOME (Short "Inl")) 1 /\
+   res <> Rerr(Rabort(Rtimeout_error)) /\
+   (∀v.
+        build_conv env.c (SOME (Short "Inl")) [v] =
+        SOME (Conv (SOME (TypeStamp "Inl" 4)) [v])) /\
+   fname <> farg /\
+   evaluate_ck ck ^st
+     (env with
+      v :=
+        nsBind "x" v
+          (nsBind "f"
+             (Closure
+                (env with
+                 v :=
+                   nsBind fname (Recclosure env [(fname,farg,fbody)] fname)
+                     env.v) farg gbody)
+             (build_rec_env
+                ^tailrec_clos
+                (env with
+                 v :=
+                   nsBind farg x
+                     (nsBind fname
+                        (Closure
+                           (env with
+                            v :=
+                              nsBind fname
+                                (Recclosure env [(fname,farg,fbody)] fname)
+                                env.v) farg gbody) env.v))
+                env')))
+     [^tailrec_body] = (st',res) ==>
+   ∃ck'.
+       evaluate_ck ck ^st
+         (env with
+          v := nsBind farg v (build_rec_env [(fname,farg,fbody)] env env.v))
+         [fbody] = (st' with clock := ck',res)`,
+  ho_match_mp_tac COMPLETE_INDUCTION >> rw[evaluate_ck_def] >>
+  pop_assum mp_tac >>
+  ntac 5 (simp[Once terminationTheory.evaluate_def]) >>
+  simp[semanticPrimitivesTheory.build_rec_env_def,semanticPrimitivesTheory.do_opapp_def,
+       Once semanticPrimitivesTheory.find_recfun_def] >>
+  rw[] >> pop_assum mp_tac >>
+  simp[Once terminationTheory.evaluate_def] >>
+  simp[evaluateTheory.dec_clock_def] >>  
+  rw[] >> pop_assum mp_tac >>
+  drule mk_single_app_evaluate_single >>
+  qmatch_goalsub_abbrev_tac `evaluate ast aenv` >>
+  disch_then(qspecl_then [`ast`,`aenv`] mp_tac) >>
+  unabbrev_all_tac >> simp[ml_progTheory.nsLookup_nsBind_compute] >>
+  simp[semanticPrimitivesTheory.build_rec_env_def,partially_evaluates_to_def] >>
+  qmatch_goalsub_abbrev_tac `evaluate ast aenv` >>
+  Cases_on `evaluate ast aenv [gbody]` >>
+  rename1 `(_,result)` >>
+  reverse(Cases_on `result`) >-
+    ((* Rerror *)
+     fs[] >> rpt strip_tac >>
+     qexists_tac `st'.clock + 1` >>
+     simp[Abbr`ast`] >>
+     drule evaluatePropsTheory.evaluate_add_to_clock >>
+     rveq >> simp[] >> disch_then(qspec_then `1` mp_tac) >>
+     simp[]) >>
+  simp[] >>
+  strip_tac >-
+    ((* Rval([Inr v]) *)
+      imp_res_tac evaluatePropsTheory.evaluate_length >>
+      fs[quantHeuristicsTheory.LIST_LENGTH_1] >>
+      rveq >>
+      imp_res_tac dest_inr_v_IMP >>
+      fs[] >> rveq >>
+      simp[Once terminationTheory.evaluate_def] >>
+      simp[namespaceTheory.nsOptBind_def] >>
+      simp[Once terminationTheory.evaluate_def] >>
+      simp[astTheory.pat_bindings_def] >>
+      simp[terminationTheory.pmatch_def] >>
+      imp_res_tac build_conv_check_IMP_nsLookup >>
+      simp[semanticPrimitivesTheory.same_type_def,semanticPrimitivesTheory.same_ctor_def] >>
+      simp[Once terminationTheory.evaluate_def] >>
+      simp[astTheory.pat_bindings_def] >>
+      simp[terminationTheory.pmatch_def] >>
+      simp[Once terminationTheory.evaluate_def] >>
+      simp[semanticPrimitivesTheory.same_type_def,semanticPrimitivesTheory.same_ctor_def] >>
+      simp[astTheory.pat_bindings_def] >>
+      simp[terminationTheory.pmatch_def] >>
+      simp[Once terminationTheory.evaluate_def] >>
+      rpt strip_tac >>
+      rveq >>
+      qexists_tac `q.clock + 1` >>
+      simp[Abbr `ast`] >>
+      drule evaluatePropsTheory.evaluate_add_to_clock >>
+      rveq >> simp[] >> disch_then(qspec_then `1` mp_tac) >>
+      simp[]
+    ) >-
+    ((* Rval([Inl v]) *)
+      imp_res_tac evaluatePropsTheory.evaluate_length >>
+      fs[quantHeuristicsTheory.LIST_LENGTH_1] >>
+      rveq >>
+      imp_res_tac dest_inl_v_IMP >>
+      fs[] >> rveq >>
+      simp[Once terminationTheory.evaluate_def] >>
+      simp[namespaceTheory.nsOptBind_def] >>
+      simp[Once terminationTheory.evaluate_def] >>
+      simp[astTheory.pat_bindings_def] >>
+      simp[terminationTheory.pmatch_def] >>
+      imp_res_tac build_conv_check_IMP_nsLookup >>
+      simp[semanticPrimitivesTheory.same_type_def,semanticPrimitivesTheory.same_ctor_def] >>
+      simp[Once terminationTheory.evaluate_def] >>
+      simp[astTheory.pat_bindings_def] >>
+      simp[terminationTheory.pmatch_def] >>
+      simp[terminationTheory.evaluate_def] >>
+      simp[semanticPrimitivesTheory.do_opapp_def,Once semanticPrimitivesTheory.find_recfun_def] >>
+      simp[Once terminationTheory.evaluate_def] >>
+      rw[] >> pop_assum mp_tac >>
+      simp[evaluateTheory.dec_clock_def] >>
+      rw[] >> pop_assum mp_tac >>
+      fs[semanticPrimitivesTheory.do_opapp_def,Once semanticPrimitivesTheory.find_recfun_def] >>
+      unabbrev_all_tac >>      
+      qmatch_goalsub_abbrev_tac
+        `evaluate
+           (ast with clock := _)
+           (aenv with
+             v := nsBind _ argv
+                   (nsBind _ funv (build_rec_env _ (_ with v := nsBind _ argx _) aenv'))
+           )` >>
+      strip_tac >>
+      first_x_assum(qspec_then `ast.clock - 2` mp_tac) >>
+      impl_tac >-
+        (unabbrev_all_tac >>
+         imp_res_tac terminationTheory.evaluate_clock >>
+         fs[]) >>
+      rpt(disch_then drule) >>
+      unabbrev_all_tac >>
+      disch_then drule >>
+      strip_tac >>
+      drule evaluatePropsTheory.evaluate_add_to_clock >>
+      simp[] >>
+      disch_then(qspec_then `1` assume_tac) >>
+      fs[evaluateTheory.dec_clock_def] >>
+      rveq >>
+      rpt(dxrule evaluatePropsTheory.evaluate_add_to_clock >>
+        simp[] >>
+        disch_then(qspec_then `1` mp_tac) >>
+        fs[] >>
+        rveq) >>
+      rpt strip_tac >>
+      fs[semanticPrimitivesTheory.state_component_equality])
+  );
+
+val evaluate_tailrec_lemma = Q.prove(
+ `!ck fbody gbody env ^st farg x fname st' res.
+   mk_single_app (SOME fname) T fbody = SOME gbody /\
+   do_con_check env.c (SOME (Short "Inr")) 1 /\
+   (∀v.
+        build_conv env.c (SOME (Short "Inr")) [v] =
+        SOME (Conv (SOME (TypeStamp "Inr" 4)) [v])) /\
+   do_con_check env.c (SOME (Short "Inl")) 1 /\
+   res <> Rerr(Rabort(Rtimeout_error)) /\
+   (∀v.
+        build_conv env.c (SOME (Short "Inl")) [v] =
+        SOME (Conv (SOME (TypeStamp "Inl" 4)) [v])) /\
+   fname <> farg /\
+   evaluate_ck ck ^st
+      (env with
+            v :=
+              nsBind farg x
+                (nsBind fname
+                   (Closure
+                      (env with
+                       v := build_rec_env [(fname,farg,fbody)] env env.v)
+                      farg gbody) env.v))
+    [App Opapp
+        [App Opapp
+           [Letrec ^tailrec_clos (Var(Short "tailrec"));
+            Var(Short fname)]; Var (Short farg)]] = (st',res) ==>
+    ∃ck'.evaluate_ck ck ^st
+         (env with
+          v := nsBind farg x (build_rec_env [(fname,farg,fbody)] env env.v))
+         [fbody] = (st' with clock := ck',res)`,
+  rpt strip_tac >>
+  fs[evaluate_ck_def] >>
+  pop_assum mp_tac >>
+  ntac 8 (simp[Once terminationTheory.evaluate_def]) >>
+  simp[semanticPrimitivesTheory.build_rec_env_def,semanticPrimitivesTheory.do_opapp_def,
+       Once semanticPrimitivesTheory.find_recfun_def] >>
+  rw[] >> pop_assum mp_tac >>
+  simp[Once terminationTheory.evaluate_def] >>
+  simp[evaluateTheory.dec_clock_def] >>  
+  rw[] >> pop_assum mp_tac >>
+  strip_tac >>
+  drule evaluate_tailrec_ind_lemma >>
+  rpt(disch_then drule) >>
+  simp[evaluate_ck_def,semanticPrimitivesTheory.build_rec_env_def] >>
+  disch_then drule >>
+  strip_tac >>
+  drule evaluatePropsTheory.evaluate_add_to_clock >>
+  simp[] >>
+  disch_then(qspec_then `2` mp_tac) >>
+  simp[semanticPrimitivesTheory.state_component_equality]);
+
+val mk_tailrec_closure_sound_basic = Q.store_thm("mk_tailrec_closure_sound_basic",
+  `!fv env . mk_tailrec_closure(Recclosure env [(fname,farg,fbody)] fname) = SOME fv
+   /\ do_con_check env.c (SOME (Short "Inr")) 1
+   /\ (!v. build_conv env.c (SOME (Short "Inr")) [v] =
+           SOME(Conv (SOME (TypeStamp "Inr" 4)) [v]))
+   /\ do_con_check env.c (SOME (Short "Inl")) 1
+   /\ (!v. build_conv env.c (SOME (Short "Inl")) [v] =
+          SOME(Conv (SOME (TypeStamp "Inl" 4)) [v]))
+   /\ fname <> farg
+   /\ app_basic p fv x H Q
+   ==> app_basic p (Recclosure env [(fname,farg,fbody)] fname) x H Q`,
+  rw[mk_tailrec_closure_def,app_basic_def] >>
+  first_x_assum drule >>
+  disch_then drule >>
+  strip_tac >>
+  asm_exists_tac >> fs[semanticPrimitivesTheory.do_opapp_def] >>
+  simp[semanticPrimitivesTheory.find_recfun_def] >>
+  asm_exists_tac >>
+  simp[] >> rveq >> Cases_on `r` >> 
+  fs[evaluate_to_heap_def] >>
+  TRY(
+    rename1 `lprefix_lub` >>
+    cheat
+  ) >>
+  qexists_tac `ck` >>
+  Q.REFINE_EXISTS_TAC `st' with clock := _` >>
+  fs[cfStoreTheory.st2heap_def] >>
+  match_mp_tac evaluate_tailrec_lemma >>
+  simp[]);
+
+val mk_tailrec_closure_sound = Q.store_thm("mk_tailrec_closure_sound",
+  `!fv env . mk_tailrec_closure(Recclosure env [(fname,farg,fbody)] fname) = SOME fv
+   /\ do_con_check env.c (SOME (Short "Inr")) 1
+   /\ (!v. build_conv env.c (SOME (Short "Inr")) [v] =
+           SOME(Conv (SOME (TypeStamp "Inr" 4)) [v]))
+   /\ do_con_check env.c (SOME (Short "Inl")) 1
+   /\ (!v. build_conv env.c (SOME (Short "Inl")) [v] =
+          SOME(Conv (SOME (TypeStamp "Inl" 4)) [v]))
+   /\ fname <> farg
+   /\ app p fv [x] H Q
+   ==> app p (Recclosure env [(fname,farg,fbody)] fname) [x] H Q`,
+  metis_tac[mk_tailrec_closure_sound_basic,app_def]);
+
 val _ = (append_prog o cfTacticsLib.process_topdecs)
   `fun repeat f x = repeat f (f x);`
 
